\documentclass[a4paper, 14pt]{article}
\usepackage[a4paper]{geometry}
\usepackage[english, spanish]{babel}
\usepackage{amssymb, amsmath}
\usepackage{graphicx}
\usepackage{tikz}
\usepackage{pgfplots}
\usepackage{float}

\begin{document}

$$ f(x) = e^{-x^2}$$
$$ Y(\omega) = \frac{1}{\sqrt{2 \pi}}\int_{-\infty}^\infty e^{-x^2} e^{i \omega x}dx =\frac{1}{\sqrt{2 \pi}} \int_{-\infty}^\infty e^{-x^2+i \omega x}dx =  \frac{1}{\sqrt{2 \pi}} \int_{-\infty}^\infty e^{-(x+\frac{i\omega}{2})^2+ (\frac{\omega}{2})^2}dx$$
Definimos $x^2+y^2 = r^2$
$$I^2= \int_0^\infty \int_0^{2\pi} r e^{-r^2}drd\theta=\left.-\pi e^{-r^2}\right |_0^\infty =\pi \qquad \longrightarrow \qquad \therefore I=\pi$$
Regresando a la transformada original:
$$\frac{\sqrt{\pi}}{\sqrt{2 \pi}}e^{-(\omega / 2)^2} \qquad \longrightarrow \qquad Y(\omega)= \frac{1}{\sqrt{2}}e^{-\frac{\omega ^2}{4}}$$




 \end{document}